logic.lean
@@ -1,38 +1,24 @@
 import .syntax .notations .evaluation .substitution .qi
 
--- validity
+-- validity is axiomatized instead of specified
 
 constant valid : vc → Prop
 notation `⊨` p: 100 := valid p
 notation σ `⊨` p: 100 := valid (vc.subst_env σ p)
+
+-- notation ⟪ P ⟫
+
 @[reducible]
 def VC(P: prop) := ∀ (σ: env), σ ⊨ P.instantiated
 notation `⟪` P `⟫`: 100 := VC P
 
--- axioms
+-- simple axioms for logical reasoning
 
 axiom valid.tru:
   ⊨ value.true
 
-axiom valid.unop {op: unop} {vₓ v: value}:
-  unop.apply op vₓ = some v
-  ↔
-  ⊨ (term.unop op vₓ ≡ v)
-
-axiom valid.binop {op: binop} {v₁ v₂ v: value}:
-  binop.apply op v₁ v₂ = some v
-  ↔
-  ⊨ (term.binop op v₁ v₂ ≡ v)
-
-axiom valid.app {vₓ v: value} {σ σ': env} {f x y: var} {R S: spec} {e: exp}:
-  (σ[x↦vₓ], e) ⟶* (σ', exp.return y) ∧
-  (σ' y = some v)
-  ↔
-  ⊨ (term.app (value.func f x R S e σ) vₓ ≡ v)
-
 axiom valid.and {P Q: vc}:
-  ⊨ P ∧
-  ⊨ Q
+  (⊨ P ∧ ⊨ Q)
   ↔
   ⊨ (P && Q)
 
@@ -41,41 +27,78 @@ axiom valid.or {P Q: vc}:
   ↔
   ⊨ (P || Q)
 
-axiom valid.mp  {P Q: vc}:
+axiom valid.implies  {P Q: vc}:
   (⊨ P → ⊨ Q)
   ↔
   ⊨ vc.implies P Q
-
-axiom valid.pre {vₓ: value} {σ: env} {f x y: var} {R S: spec} {e: exp}:
-  ⊨ vc.subst_env (σ[x↦vₓ][f↦value.func f x R S e σ]) R.to_prop.instantiated
-  ↔
-  ⊨ vc.pre (value.func f x R S e σ) vₓ
-
-axiom valid.pre₁ {vₓ: value} {op: unop}:
-  (∃v, unop.apply op vₓ = some v)
-  ↔
-  ⊨ vc.pre₁ op vₓ
-
-axiom valid.pre₂ {v₁ v₂: value} {op: binop}:
-  (∃v, binop.apply op v₁ v₂ = some v)
-  ↔
-  ⊨ vc.pre₂ op v₁ v₂
-
-axiom valid.post {vₓ: value} {σ σ': env} {f x y: var} {R S: spec} {e: exp}:
-  (σ[x↦vₓ], e) ⟶* (σ', exp.return y) ∧
-  ⊨ vc.subst_env (σ[x↦vₓ][f↦value.func f x R S e σ]) (spec.implies R S).to_prop.instantiated
-  ↔
-  ⊨ vc.post (value.func f x R S e σ) vₓ
 
 axiom valid.univ {x: var} {P: vc}:
   (∀v, ⊨ vc.subst x v P)
   ↔
   ⊨ vc.univ x P
 
+-- axioms for equality
+
+-- a term is valid if it equals true
 axiom valid.eq.true {t: term}:
-  ⊨ (t ≡ value.true)
-  ↔
   ⊨ t
+  ↔
+  ⊨ (t ≡ value.true)
+
+-- unary and binary operators are decidable, so equalities with operators are decidable
+axiom valid.eq.unop {op: unop} {vₓ v: value}:
+  unop.apply op vₓ = some v
+  ↔
+  ⊨ (term.unop op vₓ ≡ v)
+
+axiom valid.eq.binop {op: binop} {v₁ v₂ v: value}:
+  binop.apply op v₁ v₂ = some v
+  ↔
+  ⊨ (term.binop op v₁ v₂ ≡ v)
+
+-- The following equality axiom is non-standard and makes validity undecidable.
+-- It is only used in the preservation proof of e-return and in no other lemmas.
+-- The logic treats `f(x)` uninterpreted, so there is no way to derive it naturally.
+-- However, given a complete evaluation derivation of a function call, we can add the
+-- equality `f(x)=y` as new axiom for closed values f, x, y and the resulting set
+-- of axioms is still sound due to deterministic evaluation.
+axiom valid.eq.app {vₓ v: value} {σ σ': env} {f x y: var} {R S: spec} {e: exp}:
+  (σ[x↦vₓ], e) ⟶* (σ', exp.return y) ∧
+  (σ' y = some v)
+  →
+  ⊨ (term.app (value.func f x R S e σ) vₓ ≡ v)
+
+-- can write pre₁ and pre₂ to check domain of operators
+
+axiom valid.pre₁ {vₓ: value} {op: unop}:
+  option.is_some (unop.apply op vₓ)
+  ↔
+  ⊨ vc.pre₁ op vₓ
+
+axiom valid.pre₂ {v₁ v₂: value} {op: binop}:
+  option.is_some (binop.apply op v₁ v₂)
+  ↔
+  ⊨ vc.pre₂ op v₁ v₂
+
+-- can write pre and post to extract pre- and postcondition of function values
+
+axiom valid.pre {vₓ: value} {σ: env} {f x: var} {R S: spec} {e: exp}:
+  ⊨ vc.subst_env (σ[x↦vₓ][f↦value.func f x R S e σ]) R.to_prop.instantiated
+  ↔
+  ⊨ vc.pre (value.func f x R S e σ) vₓ
+
+axiom valid.post {vₓ: value} {σ σ': env} {f x y: var} {R S: spec} {e: exp}:
+  ⊨ vc.subst_env (σ[x↦vₓ][f↦value.func f x R S e σ]) S.to_prop.instantiated
+  ↔
+  ⊨ vc.post (value.func f x R S e σ) vₓ
+
+-- axioms about instantiations
+
+--  inst(P)   ⇒   inst_n(P)
+--         ⇘    ⇗  
+--     ⇑      P      ⇓
+--         ⇗    ⇘ 
+-- erased(P)     erased_n(P)
 
 axiom valid_env.instantiated_of_erased {σ: env} {P: prop}:
   σ ⊨ P.erased →
@@ -89,6 +112,8 @@ axiom valid_env.erased_n_of_instantiated_n {σ: env} {P: prop}:
   σ ⊨ P.instantiated_n →
   σ ⊨ P.erased_n
 
+-- if a conjunction or disjunciton is valid without cross-instantiations
+-- then it remains valid, as potential new instantiations are in negative positions
 axiom valid_env.instantiated_and {σ: env} {P Q: prop}:
   σ ⊨ (P.instantiated && Q.instantiated) →
   σ ⊨ (P && Q).instantiated
@@ -96,6 +121,16 @@ axiom valid_env.instantiated_and {σ: env} {P Q: prop}:
 axiom valid_env.instantiated_or {σ: env} {P Q: prop}:
   σ ⊨ (P.instantiated || Q.instantiated) →
   σ ⊨ (P || Q).instantiated
+
+-- if P and P' have the exact same triggers and quantifiers, then
+-- any instantiation with an arbitrary propostion Q are also the same,
+-- so if (P') implies (P) without cross-instantiations,
+-- then (P' ∧ Q) implies (P ∧ Q) without cross-instantiations
+axiom valid_env.strengthen_without_instantiations {σ: env} {P P' Q: prop}:
+  (calls P = calls P') →
+  (quantifiers P = quantifiers P') →
+  σ ⊨ vc.implies P'.instantiated_n P.instantiated_n →
+  σ ⊨ vc.implies (P' && Q).instantiated_n (P && Q).instantiated_n
 
 -- lemmas
 
@@ -128,8 +163,8 @@ lemma valid.refl {v: value}: ⊨ (v ≡ v) :=
                                   (classical.prop_decidable (v = v))
                                   value value.true value.false, by unfold binop.apply,
   have binop.apply binop.eq v v = value.true, by simp[this],
-  have ⊨ ((v ≡ v) ≡ value.true), from valid.binop.mp this,
-  show ⊨ (v ≡ v), from valid.eq.true.mp this
+  have ⊨ ((v ≡ v) ≡ value.true), from valid.eq.binop.mp this,
+  show ⊨ (v ≡ v), from valid.eq.true.mpr this
 
 lemma valid_env.true {σ: env}: σ ⊨ value.true :=
   have h1: ⊨ value.true, from valid.tru,
@@ -158,11 +193,11 @@ lemma valid_env.mp {σ: env} {P Q: vc}: σ ⊨ vc.implies P Q → σ ⊨ P → �
   have vc.subst_env σ P.not = (vc.subst_env σ P).not, from vc.subst_env.not,
   have ⊨ ((vc.subst_env σ P).not || vc.subst_env σ Q), from this ▸ h,
   have ⊨ vc.implies (vc.subst_env σ P) (vc.subst_env σ Q), from this,
-  show σ ⊨ Q, from valid.mp.mpr this p
+  show σ ⊨ Q, from valid.implies.mpr this p
 
 lemma valid_env.mpr {σ: env} {P Q: vc}: (σ ⊨ P → σ ⊨ Q) → σ ⊨ vc.implies P Q :=
   assume : (σ ⊨ P → σ ⊨ Q),
-  have ⊨ vc.implies (vc.subst_env σ P) (vc.subst_env σ Q), from valid.mp.mp this,
+  have ⊨ vc.implies (vc.subst_env σ P) (vc.subst_env σ Q), from valid.implies.mp this,
   have h1: ⊨ vc.or (vc.subst_env σ P).not (vc.subst_env σ Q), from this,
   have vc.subst_env σ P.not = (vc.subst_env σ P).not, from vc.subst_env.not,
   have h2: ⊨ vc.or (vc.subst_env σ P.not) (vc.subst_env σ Q), from this.symm ▸ h1,
@@ -170,40 +205,3 @@ lemma valid_env.mpr {σ: env} {P Q: vc}: (σ ⊨ P → σ ⊨ Q) → σ ⊨ vc.i
   from vc.subst_env.or,
   have ⊨ vc.subst_env σ (P.not || Q), from this.symm ▸ h2,
   show σ ⊨ vc.implies P Q, from this
-
-lemma history_valid {H: callhistory}: ⟪calls_to_prop H⟫ :=
-  assume σ: env,
-  begin
-    induction H,
-    case list.nil { from (
-      have h1: σ ⊨ value.true, from valid_env.true,
-      have (prop.term value.true).erased = vc.term value.true, by unfold prop.erased,
-      have σ ⊨ (prop.term value.true).erased, from this ▸ h1,
-      have h2: σ ⊨ (prop.term value.true).instantiated, from valid_env.instantiated_of_erased this,
-      have calls_to_prop list.nil = value.true, by unfold calls_to_prop,
-      show σ ⊨ (calls_to_prop list.nil).instantiated, from this ▸ h2
-    )},
-    case list.cons h rest ih {
-      cases h,
-      case historyitem.nop { from (
-        have h2: σ ⊨ (calls_to_prop rest).instantiated, from ih,
-        have calls_to_prop (historyitem.nop :: rest) = calls_to_prop rest, by unfold calls_to_prop,
-        show σ ⊨ (calls_to_prop (historyitem.nop :: rest)).instantiated, from this.symm ▸ h2
-      )},
-      case historyitem.call f x R S e σ₂ v { from (
-        have h1: σ ⊨ value.true, from valid_env.true,
-        have (prop.call (value.func f x R S e σ₂) v).erased = vc.term value.true, by unfold prop.erased,
-        have σ ⊨ (prop.call (value.func f x R S e σ₂) v).erased, from this ▸ h1,
-        have h2: σ ⊨ (prop.call (value.func f x R S e σ₂) v).instantiated, from valid_env.instantiated_of_erased this,
-        have h3: σ ⊨ (calls_to_prop rest).instantiated, from ih,
-        have σ ⊨ ((prop.call (value.func f x R S e σ₂) v).instantiated && (calls_to_prop rest).instantiated),
-        from valid_env.and h2 h3,
-        have h4: σ ⊨ (prop.call (value.func f x R S e σ₂) v && calls_to_prop rest).instantiated,
-        from valid_env.instantiated_and this,
-        have calls_to_prop (call f x R S e σ₂ v :: rest)
-          = prop.call (value.func f x R S e σ₂) v && calls_to_prop rest,
-        by unfold calls_to_prop,
-        show σ ⊨ (calls_to_prop (call f x R S e σ₂ v :: rest)).instantiated, from this ▸ h4
-      )}
-    }
-  end
